theories/Constructions/TypeSystem.v
@@ -13,128 +13,141 @@ Require Import Local.Constructions.Conversion.
 
 Import ListNotations.
 
-Inductive typing: env -> relation term :=
-  (*
-           |- G
-    --------------------
-      G |- Prop : Type
-  *)
-  | typing_prop:
-    forall g,
-    valid_env g ->
-    typing g (sort prop) (sort type)
-  (*
-      (x: T) or (x = e: T) in G
-    -----------------------------
-             G |- x : T
-  *)
-  | typing_bound:
-    forall g n d t u,
-    valid_env g ->
-    item (d, t) g n ->
-    u = lift (1 + n) 0 t ->
-    typing g (bound n) u
-  (*
-       G, X: T |- U : s
-    ----------------------
-      G |- Pi X: T.U : s
-  *)
-  | typing_pi:
-    forall g t u s,
-    typing (decl_var t :: g) u (sort s) ->
-    typing g (pi t u) (sort s)
-  (*
-          G, x: T |- e: U
-    ----------------------------
-      G |- \x: T.e : Pi x: T.U
-  *)
-  | typing_abs:
-    forall g t e u,
-    typing (decl_var t :: g) e u ->
-    typing g (abstraction t e) (pi t u)
-  (*
-      G |- f : Pi x: T.U     G |- e : T
-    -------------------------------------
-              G |- f e : U[e/x]
-  *)
-  | typing_app:
-    forall g f e t u,
-    typing g f (pi t u) ->
-    typing g e t ->
-    typing g (application f e) (subst e 0 u)
-  (*
-      G |- e : T     G, x = e: T |- f : U
-    ---------------------------------------
-        G |- let x = e: T in f : U[e/x]
-  *)
-  | typing_def:
-    forall g e f t u,
-    typing g e t ->
-    typing (decl_def e t :: g) f u ->
-    typing g (definition e t f) (subst e 0 u)
-  (*
-      G |- e : T     G |- U : s     G |- T = U
-    --------------------------------------------
-                     G |- e : U
-  *)
-  | typing_conv:
-    forall g e t u s,
-    typing g e t ->
-    typing g u (sort s) ->
-    conv g t u ->
-    typing g e u
+(* QUANTIFY OVER EQUALITY
+   MAKE OBSERVATIONAL EQUALITY NOT RELY ON BETA BUT ITSELF
+   On the paper we can discuss the choice of full beta for CBV *)
 
-with valid_env: env -> Prop :=
-  (*
-    --------
-      |- .
-  *)
-  | valid_env_nil:
-    valid_env []
-  (*
-      |- G     G |- T: s
-    -----------------------
-          |- G, x: T
-  *)
-  | valid_env_var:
-    forall g t s,
-    valid_env g ->
-    typing g t (sort s) ->
-    valid_env (decl_var t :: g)
-  (*
-      |- G     G |- e : T     G |- T : s
-    --------------------------------------
-              |- G, x = e: T
-  *)
-  | valid_env_def:
-    forall g e t s,
-    valid_env g ->
-    typing g e t ->
-    typing g t (sort s) ->
-    valid_env (decl_def e t :: g).
+Definition type_equality: Type :=
+  env -> term -> relation term.
 
-(* Coq term: [\X: Prop.\x: X.x]. *)
-Example polymorphic_id_term: term :=
-  abstraction (sort prop) (abstraction (bound 0) (bound 0)).
+Section TypeSystem.
 
-(* Coq term: [Pi X: Prop.X -> X]. *)
-Example polymorphic_id_type: term :=
-  pi (sort prop) (pi (bound 0) (bound 1)).
+  Variable R: type_equality.
 
-(* Let's check typeability. *)
-Goal
-  typing [] polymorphic_id_term polymorphic_id_type.
-Proof.
-  simpl.
-  repeat econstructor.
-  (* Of course! *)
-  now vm_compute.
-Qed.
+  Inductive typing: env -> relation term :=
+    (*
+             |- G
+      --------------------
+        G |- Prop : Type
+    *)
+    | typing_prop:
+      forall g,
+      valid_env g ->
+      typing g (sort prop) (sort type)
+    (*
+        (x: T) or (x = e: T) in G
+      -----------------------------
+               G |- x : T
+    *)
+    | typing_bound:
+      forall g n d t u,
+      valid_env g ->
+      item (d, t) g n ->
+      u = lift (1 + n) 0 t ->
+      typing g (bound n) u
+    (*
+         G, X: T |- U : s
+      ----------------------
+        G |- Pi X: T.U : s
+    *)
+    | typing_pi:
+      forall g t u s,
+      typing (decl_var t :: g) u (sort s) ->
+      typing g (pi t u) (sort s)
+    (*
+            G, x: T |- e: U
+      ----------------------------
+        G |- \x: T.e : Pi x: T.U
+    *)
+    | typing_abs:
+      forall g t e u,
+      typing (decl_var t :: g) e u ->
+      typing g (abstraction t e) (pi t u)
+    (*
+        G |- f : Pi x: T.U     G |- e : T
+      -------------------------------------
+                G |- f e : U[e/x]
+    *)
+    | typing_app:
+      forall g f e t u,
+      typing g f (pi t u) ->
+      typing g e t ->
+      typing g (application f e) (subst e 0 u)
+    (*
+        G |- e : T     G, x = e: T |- f : U
+      ---------------------------------------
+          G |- let x = e: T in f : U[e/x]
+    *)
+    | typing_def:
+      forall g e f t u,
+      typing g e t ->
+      typing (decl_def e t :: g) f u ->
+      typing g (definition e t f) (subst e 0 u)
+    (*
+        G |- e : T     G |- U : s     G |- T R U : s
+      ------------------------------------------------
+                         G |- e : U
+    *)
+    | typing_conv:
+      forall g e t u s,
+      typing g e t ->
+      typing g u (sort s) ->
+      R g (sort s) t u ->
+      typing g e u
+
+  with valid_env: env -> Prop :=
+    (*
+      --------
+        |- .
+    *)
+    | valid_env_nil:
+      valid_env []
+    (*
+        |- G     G |- T: s
+      -----------------------
+            |- G, x: T
+    *)
+    | valid_env_var:
+      forall g t s,
+      valid_env g ->
+      typing g t (sort s) ->
+      valid_env (decl_var t :: g)
+    (*
+        |- G     G |- e : T     G |- T : s
+      --------------------------------------
+                |- G, x = e: T
+    *)
+    | valid_env_def:
+      forall g e t s,
+      valid_env g ->
+      typing g e t ->
+      typing g t (sort s) ->
+      valid_env (decl_def e t :: g).
+
+  (* Coq term: [\X: Prop.\x: X.x]. *)
+  Example polymorphic_id_term: term :=
+    abstraction (sort prop) (abstraction (bound 0) (bound 0)).
+
+  (* Coq term: [Pi X: Prop.X -> X]. *)
+  Example polymorphic_id_type: term :=
+    pi (sort prop) (pi (bound 0) (bound 1)).
+
+  (* Let's check typeability. *)
+  Goal
+    typing [] polymorphic_id_term polymorphic_id_type.
+  Proof.
+    simpl.
+    repeat econstructor.
+    (* Of course! *)
+    now vm_compute.
+  Qed.
+
+End TypeSystem.
 
 Lemma valid_env_typing:
-  forall g e t,
-  typing g e t ->
-  valid_env g.
+  forall R g e t,
+  typing R g e t ->
+  valid_env R g.
 Proof.
   induction 1.
   - assumption.
